Two test examples HO

io/Compiler.Examples.fst
@@ -68,7 +68,7 @@ let ex1 : src_interface = {
   ct_rcs = Node (| unit, resexn file_descr, ex1_ct_rc |) Leaf Leaf;
 
   ct_importable = (fun fl -> 
-    safe_importable_arrow_pre_post_args unit _ _ _ ex1_c1post ex1_c2post);
+    safe_importable_arrow_pre_post_args_res _ _ ex1_c1post ex1_c2post #exportable_unit #importable_file_descr);
   p_post = (fun _ _ _ lt -> (forall fd'. ~((EOpenfile "/etc/passwd" fd') `List.memP` lt)));
 }
 
@@ -87,43 +87,48 @@ let ex1_ctx_t #fl io_acts () : IIOpi (resexn file_descr) fl (comp_int_src_tgt ex
   io_acts Openfile "/etc/passwd"
 
 (** ** Example 2 - HO left 1 **)
+let ex2_pi : monitorable_prop = (fun _ _ _ -> true)
+val ex2_stronger_pis : squash (forall h lt. enforced_locally ex2_pi h lt ==> enforced_locally ex2_pi h lt)
+let ex2_stronger_pis = ()
 
-let ex3_pi : monitorable_prop = (fun _ _ _ -> true)
-let ex3_post = (fun h (rfd:resexn file_descr) lt -> Inl? rfd ==> is_open (Inl?.v rfd) (rev lt @ h))
+let ex2_cb (fl:erased tflag) = (fd:file_descr -> IIO (resexn unit) fl (fun h -> is_open fd h) (fun _ _ lt -> lt == []))
+let ex2_post = (fun _ h (rfd:resexn file_descr) lt -> Inl? rfd ==> is_open (Inl?.v rfd) (rev lt @ h))
+let ex2_ct (fl:erased tflag) = (cb:ex2_cb fl) -> IIO (resexn file_descr) fl (fun _ -> True) (ex2_post cb)
 
-assume val ex3_stronger_pis : squash (forall h lt. enforced_locally ex3_pi h lt ==> enforced_locally ex3_pi h lt)
-
-let ex3_rcs : tree pck_rc =  
+let ex2_rcs : tree pck_rc =  
   Node (| unit, resexn file_descr, (fun () h (rfd:resexn file_descr) lt -> Inl? rfd && (is_open (Inl?.v rfd) (rev lt @ h))) |) 
      (Node (| file_descr, unit, (fun fd h _ _ -> is_open fd h) |) Leaf Leaf)
      Leaf
   
-assume val ex3_c1post : squash (forall h lt. enforced_locally ex3_pi h lt ==> (exists (rfd:resexn file_descr). Inl? rfd ==> is_open (Inl?.v rfd) (rev lt @ h)))
-val ex3_c2post : squash (forall h (rfd:resexn file_descr) lt. Inl? rfd && (is_open (Inl?.v rfd) (rev lt @ h)) ==> (Inl? rfd ==> is_open (Inl?.v rfd) (rev lt @ h)))
-let ex3_c2post = ()
+assume val ex2_c1post : #a:Type -> squash (forall (x:a) h lt. enforced_locally ex2_pi h lt ==> (exists r. ex2_post x h r lt))
 
-let ex3 : src_interface = {
-  spec_pi = ex3_pi;
-  inst_pi = ex3_pi;
-  inst_pi_stronger_spec_pi = ex3_stronger_pis;
+val ex2_c2post : #a:Type -> squash (forall (x:a) h r lt. enforced_locally ex2_pi h lt /\ ((Mkdtuple3?._3 (root ex2_rcs)) () h r lt) ==> ex2_post x h r lt)
+let ex2_c2post #a = ()
 
-  ct = (fun fl -> (fd:file_descr -> IIO (resexn unit) fl (fun h -> is_open fd h) (fun _ _ lt -> lt == [])) -> IIO (resexn file_descr) fl (fun _ -> True) ex3_post);
-  ct_rcs = ex3_rcs;
+let ex2_ct_importable (fl:erased tflag) : safe_importable (ex2_ct fl) ex2_pi ex2_rcs fl = 
+  let exportable_cb = exportable_arrow_pre_post_args file_descr unit #ex2_pi #(left ex2_rcs) #fl (fun fd h -> is_open fd h) (fun fd _ _ lt -> lt == []) in
+  safe_importable_arrow_pre_post_res
+    (fun _ _ -> True)  (** pre **)
+    ex2_post       (** post **)
+    (ex2_c1post #(ex2_cb fl))
+    (ex2_c2post #(ex2_cb fl))
+    #exportable_cb
+    #importable_file_descr
 
-  ct_importable = (fun fl -> 
-    let exportable_cb = exportable_arrow_pre_post_args file_descr unit #ex3_pi #(left ex3_rcs) #fl (fun fd h -> is_open fd h) (fun fd _ _ lt -> lt == []) in
-    safe_importable_arrow_pre_post exportable_cb importable_file_descr (fun _ -> True) (fun h rfd lt -> Inl? rfd ==> is_open (Inl?.v rfd) (rev lt @ h)) ex3_c1post ex3_c2post);
-
+[@@ (postprocess_with (fun () -> norm [delta_only [`%ex2_ct; `%ex2_cb;`%ex2_ct_importable]]; trefl ()))]
+let ex2 : src_interface = {
+  spec_pi = ex2_pi; inst_pi = ex2_pi; inst_pi_stronger_spec_pi = ex2_stronger_pis;
+  ct = ex2_ct; ct_rcs = ex2_rcs; ct_importable = ex2_ct_importable; 
   p_post = (fun _ _ _ _ -> True);
 }
 
-val ex3_prog : prog_src ex3
-let ex3_prog #fl ctx args =
+val ex2_prog : prog_src ex2
+let ex2_prog #fl ctx args =
   let _ = ctx (fun fd -> Inl ()) in
-  0
+  (** return exit code **) 0
 
-val ex3_ctx : ctx_src ex3 
-let ex3_ctx #fl io_acts eff_rcs cb : IIO (resexn file_descr) fl (fun _ -> True) (fun h rfd lt -> Inl? rfd ==> is_open (Inl?.v rfd) (rev lt @ h)) = 
+val ex2_ctx : ctx_src ex2 
+let ex2_ctx #fl io_acts eff_rcs cb : IIO (resexn file_descr) fl (fun _ -> True) (fun h rfd lt -> Inl? rfd ==> is_open (Inl?.v rfd) (rev lt @ h)) = 
   let post1 = root eff_rcs in
   let (| _, pre1 |) = root (left eff_rcs) in 
   let rfd = io_acts Openfile "/etc/passwd" in
@@ -131,8 +136,8 @@ let ex3_ctx #fl io_acts eff_rcs cb : IIO (resexn file_descr) fl (fun _ -> True) 
   | Inl fd -> let _ = pre1 fd in rfd
   | _ -> rfd
 
-val ex3_ctx_t : ctx_tgt (comp_int_src_tgt ex3)
-let ex3_ctx_t #fl io_acts cb : IIOpi (resexn file_descr) fl (comp_int_src_tgt ex3).spec_pi = 
+val ex2_ctx_t : ctx_tgt (comp_int_src_tgt ex2)
+let ex2_ctx_t #fl io_acts cb : IIOpi (resexn file_descr) fl (comp_int_src_tgt ex2).spec_pi = 
   let rfd = io_acts Openfile "/etc/passwd" in
   match rfd with
   | Inl fd -> begin
@@ -141,3 +146,70 @@ let ex3_ctx_t #fl io_acts cb : IIOpi (resexn file_descr) fl (comp_int_src_tgt ex
     rfd
   end
   | _ -> rfd
+
+(** ** Example 3 - HO right 1 **)
+let ex3_pi : monitorable_prop = (fun _ _ _ -> true)
+val ex3_stronger_pis : squash (forall h lt. enforced_locally ex3_pi h lt ==> enforced_locally ex3_pi h lt)
+let ex3_stronger_pis = ()
+
+let ex3_cb (fl:erased tflag) = (fd:file_descr -> IIO (resexn unit) fl (fun h -> True) (fun _ _ lt -> True))
+let ex3_post #a = (fun (x:file_descr) h (r:a) lt -> True)
+let ex3_ct (fl:erased tflag) = x:file_descr -> IIO (resexn (ex3_cb fl)) fl (fun _ -> True) (ex3_post x)
+
+let ex3_rcs : tree pck_rc =  
+  Node (| file_descr, unit, (fun x h r lt -> true) |) 
+     Leaf
+     (Node (| file_descr, resexn unit, (fun fd h _ _ -> true) |) Leaf Leaf)
+
+let ex3_cb_importable (fl:erased tflag) : safe_importable (ex3_cb fl) ex3_pi (right ex3_rcs) fl = 
+  safe_importable_arrow_pre_post_args_res
+    #file_descr #unit
+    #ex3_pi
+    #(right ex3_rcs)
+    #fl
+    (fun fd h -> True)
+    (fun fd _ _ lt -> True)
+    ()
+    ()
+    #exportable_file_descr
+    #importable_unit
+  
+assume val ex3_c1post : #a:Type -> squash (forall x h lt. enforced_locally ex3_pi h lt ==> (exists (r:a). ex3_post x h r lt))
+//let ex3_c1post #a = () 
+val ex3_c2post : #a:Type -> squash (forall x h (r:a) lt. enforced_locally ex3_pi h lt /\ ((Mkdtuple3?._3 (root ex3_rcs)) x h () lt) ==> ex3_post x h r lt)
+let ex3_c2post #a = ()
+
+let ex3_ct_importable (fl:erased tflag) : safe_importable (ex3_ct fl) ex3_pi ex3_rcs fl = 
+  safe_importable_arrow_pre_post_args
+    #file_descr #(ex3_cb fl) #ex3_pi #ex3_rcs #fl
+    (fun _ _ -> True)  (** pre **)
+    ex3_post       (** post **)
+    (ex3_c1post #(ex3_cb fl))
+    (ex3_c2post #(ex3_cb fl))
+    #exportable_file_descr
+    #(safe_importable_is_importable (ex3_cb_importable fl))
+
+[@@ (postprocess_with (fun () -> norm [delta_only [`%ex3_ct; `%ex3_cb;`%ex3_ct_importable;`%ex3_cb_importable;`%safe_importable_is_importable]]; trefl ()))]
+let ex3 : src_interface = {
+  spec_pi = ex3_pi; inst_pi = ex3_pi; inst_pi_stronger_spec_pi = ex3_stronger_pis;
+  ct = ex3_ct; ct_rcs = ex3_rcs; ct_importable = ex3_ct_importable; 
+  p_post = (fun _ _ _ _ -> True);
+}
+
+val ex3_prog : prog_src ex3
+let ex3_prog #fl ctx args : IIO int (IOActions + fl) (fun _ -> True) (fun _ _ _ -> True) =
+  match static_cmd Openfile "test.txt" with
+  | Inl fd -> begin
+    match ctx fd with
+    | Inl cb -> let _ : resexn unit = cb fd in 0
+    | Inr err -> -1
+    end
+  | Inr err -> -1
+
+val ex3_ctx : ctx_src ex3 
+let ex3_ctx #fl io_acts eff_rcs fd = 
+  Inl (fun (fd:file_descr) -> Inl ())
+
+val ex3_ctx_t : ctx_tgt (comp_int_src_tgt ex3)
+let ex3_ctx_t #fl io_acts fd : IIOpi (resexn (file_descr -> IIOpi (resexn unit) fl ex3_pi)) fl ex3_pi = 
+  Inl (fun (fd:file_descr) -> Inl ())
